pulse/ulib/LowStar.RST.Loops.fst
@@ -12,29 +12,11 @@ module U32 = FStar.UInt32
 
 open FStar.Mul
 
-let rec while res inv guard test body =
+inline_for_extraction let rec while res inv guard test body =
   if test () then begin
     body ();
     while res inv guard test body
   end
-
-
-inline_for_extraction val for:
-  start:U32.t ->
-  finish:U32.t{U32.v finish >= U32.v start} ->
-  context: resource ->
-  loop_inv:(h:imem (inv (context)) -> nat -> Type0) ->
-  f:(i:U32.t{U32.(v start <= v i /\ v i < v finish)} -> RST unit
-    (context)
-    (fun _ -> context)
-    (requires (fun h -> loop_inv h (U32.v i)))
-    (ensures (fun h_1 _ h_2 -> U32.(loop_inv h_1 (v i) /\ loop_inv h_2 (v i + 1))))
-  ) ->
-  RST unit
-    (context)
-    (fun _ -> context)
-    (requires (fun h -> loop_inv h (U32.v start)))
-    (ensures (fun _ _ h_2 -> loop_inv h_2 (U32.v finish)))
 
 inline_for_extraction let rec for start finish context loop_inv f =
   if start = finish then
@@ -43,71 +25,3 @@ inline_for_extraction let rec for start finish context loop_inv f =
     f start;
     for (U32.(start +^ 1ul)) finish context loop_inv f
   end
-
-val iteri:
-  #a: Type0 ->
-  b: A.array a ->
-  context: resource ->
-  loop_inv:(h:imem (inv (context)) -> nat -> Type) ->
-  f: (i:U32.t{U32.v i < A.vlength b} -> x:a -> RST unit
-    (context)
-    (fun _ -> context)
-    (fun h0 -> loop_inv h0 (U32.v i))
-    (fun h0 _ h1 -> loop_inv h0 (U32.v i) /\ loop_inv h1 (U32.v i + 1))
-  ) ->
-  RST unit
-    (R.(AR.array_resource b <*> context))
-    (fun _ -> R.(AR.array_resource b <*> context))
-    (fun h0 -> loop_inv h0 0)
-    (fun h0 _ h1 -> loop_inv h1 (A.vlength b) /\
-      R.sel (R.view_of (AR.array_resource b)) h0 ==
-      R.sel (R.view_of (AR.array_resource b)) h1
-    )
-
-let iteri #a b context loop_inv f =
-  (**) let hinit = HST.get () in
-  (**) let correct_inv = fun h i -> loop_inv h i /\
-  (**)  R.sel (R.view_of (AR.array_resource b)) hinit ==
-  (**)  R.sel (R.view_of (AR.array_resource b)) h
-  (**) in
-  let correct_f (i:U32.t{U32.(0 <= v i /\ v i < A.vlength b)})
-    : RST unit
-      (R.(AR.array_resource b) <*> context)
-      (fun _ -> R.(AR.array_resource b <*> context))
-      (requires (fun h0 ->
-        correct_inv h0 (U32.v i)
-      ))
-      (ensures (fun h0 _ h1 ->
-        U32.(correct_inv h0 (v i) /\ correct_inv h1 (v i + 1))
-      ))
-  =
-    let x = RST.rst_frame
-      (R.(AR.array_resource b <*> context))
-      (fun _ -> R.(AR.array_resource b <*> context))
-      (fun _ -> AR.index b i)
-    in
-    let f' () : RST unit // TODO: figure out why we cannot remove this superfluous let-binding
-      (context)
-      (fun _ -> context)
-      (fun h0 ->  loop_inv h0 (U32.v i))
-      (fun h0 _ h1 -> loop_inv h0 (U32.v i) /\ loop_inv h1 (U32.v i + 1))
-      =
-      f i x
-    in
-     RST.rst_frame
-       (AR.array_resource b <*> context)
-       #(context)
-       #unit
-       (fun _ -> R.(AR.array_resource b <*> context))
-       #(fun _ -> context)
-       #(AR.array_resource b)
-       #(fun h0 ->  loop_inv h0 (U32.v i))
-       #(fun h0 _ h1 -> loop_inv h0 (U32.v i) /\ loop_inv h1 (U32.v i + 1))
-       f'
-  in
-  for
-    0ul
-    (A.length b)
-    R.(AR.array_resource b <*> context)
-    correct_inv
-    correct_f
