pulse/ulib/LowStar.RST.Loops.fsti
@@ -9,23 +9,44 @@ module U32 = FStar.UInt32
 open FStar.Mul
 
 inline_for_extraction
-val while:
-    res:resource
-  -> inv: (res.t -> Type0)
-  -> guard: (res.t -> GTot bool)
-  -> test: (unit -> RST bool
-                      (res)
-                      (fun _ -> res)
-                      (requires fun h -> inv (sel (view_of res) h))
-                      (ensures fun h0 b h1 -> b == guard (sel (view_of res) h0) /\
-                               sel (view_of res) h0 == sel (view_of res) h1))
-  -> body: (unit -> RST unit
-                      (res)
-                      (fun _ -> res)
-                      (requires fun h -> guard (sel (view_of res) h))
-                      (ensures fun _ _ h -> inv (sel (view_of res) h)))
-  -> RST unit
-        (res)
-        (fun _ -> res)
-        (requires fun h -> inv (sel (view_of res) h))
-        (ensures fun _ _ h -> inv (sel (view_of res) h) /\ ~(guard (sel (view_of res) h)))
+val while
+  (res:resource)
+  (inv: (res.t -> Type0))
+  (guard: (res.t -> GTot bool))
+  (test: (unit -> RST bool
+    res
+    (fun _ -> res)
+    (requires fun old -> inv (old res))
+    (ensures fun old b modern ->
+      b == guard (old res) /\
+      old res == modern res)
+  ))
+  (body: (unit -> RST unit
+    res
+    (fun _ -> res)
+    (requires fun old -> guard (old res) /\ inv (old res))
+    (ensures fun old _ modern -> inv (modern res))
+  ))
+  : RST unit
+    res
+    (fun _ -> res)
+    (requires fun old -> inv (old res))
+    (ensures fun _ _ modern -> inv (modern res) /\ ~(guard (modern res)))
+
+inline_for_extraction
+val for
+  (start:U32.t)
+  (finish:U32.t{U32.v finish >= U32.v start})
+  (context: resource)
+  (loop_inv: (context.t -> nat -> Type0))
+  (f:(i:U32.t{U32.(v start <= v i /\ v i < v finish)} -> RST unit
+    (context)
+    (fun _ -> context)
+    (requires (fun old -> loop_inv (old context) (U32.v i)))
+    (ensures (fun old _ modern -> U32.(loop_inv (old context) (v i) /\ loop_inv (modern context) (v i + 1))))
+  ))
+  : RST unit
+    (context)
+    (fun _ -> context)
+    (requires (fun old -> loop_inv (old context) (U32.v start)))
+    (ensures (fun _ _ modern -> loop_inv (modern context) (U32.v finish)))
